cfrontend/BeePL_sem_proofs.v
@@ -1,0 +1,129 @@
+Require Import String ZArith Coq.FSets.FMapAVL Coq.Structures.OrderedTypeEx FunInd.
+Require Import Coq.FSets.FSetProperties Coq.FSets.FMapFacts FMaps FSetAVL Nat PeanoNat Linking.
+Require Import Coq.Arith.EqNat Coq.ZArith.Int Integers AST Maps Linking Ctypes Smallstep.
+Require Import Globalenvs Cop BeePL_aux BeePL_mem BeeTypes BeePL Csyntax.
+Require Import Initializersproof Cstrategy BeePL_auxlemmas Coqlib Errors SimplExpr Events.
+
+From mathcomp Require Import all_ssreflect. 
+
+Section Big_Step_Semantics.
+
+Variable (ge : genv).
+
+(* Big step semantics without lv, rv, or context *)
+Inductive bsem_expr : vmap -> Memory.mem -> BeePL.expr -> Memory.mem -> vmap -> value -> Prop := 
+| bsem_value : forall vm m v t,
+               bsem_expr vm m (Val v t) m vm v
+| bsem_lvar : forall vm m x t l ofs h a v,
+             vm!(x.(vname)) = Some (l, Reftype h (Bprim t) a) -> 
+             deref_addr ge x.(vtype) m l ofs Full v ->
+             bsem_expr vm m (Var x) m vm v
+| bsem_gbvar : forall vm m x l ofs v,
+               vm!(x.(vname)) = None ->
+               Genv.find_symbol ge x.(vname) = Some l -> 
+               deref_addr ge x.(vtype) m l ofs Full v ->
+               bsem_expr vm m (Var x) m vm v
+| bsem_consti : forall vm m i t,
+                bsem_expr vm m (Const (ConsInt i) t) m vm (Vint i)
+| bsem_constl : forall vm m i t, 
+                bsem_expr vm m (Const (ConsLong i) t) m vm (Vint64 i)
+| bsem_constu : forall vm m,
+                bsem_expr vm m (Const (ConsUnit) (Ptype Tunit)) m vm (Vunit)
+| bsem_appr : forall vm1 vm2 m1 e es t l fd m2 m3 m4 m5 m6 vs rv vm3 vm4 vm5,
+              bsem_expr vm1 m1 e m2 vm2 (Vloc l Ptrofs.zero) ->
+              Genv.find_funct ge (transBeePL_value_cvalue (Vloc l Ptrofs.zero)) = Some (Internal fd) ->
+              BeePL.type_of_fundef (Internal fd) = 
+              Ftype (typeof_exprs es) (get_effect_fundef (Internal fd)) (get_rt_fundef (Internal fd)) ->
+              list_norepet (fd.(fn_args) ++ fd.(BeePL.fn_vars)) ->
+              alloc_variables vm2 m2 (fd.(fn_args) ++ fd.(BeePL.fn_vars)) vm3 m3 -> 
+              bsem_exprs vm3 m3 es m4 vm4 vs ->
+              typeof_values vs (wtypes_of_types (extract_types_vinfos fd.(fn_args))) ->
+              bind_variables ge vm4 m4 fd.(fn_args) vs m5  ->
+              bsem_expr vm4 m5 fd.(BeePL.fn_body) m6 vm5 rv -> 
+              bsem_expr vm1 m1 (App e es t) m6 vm5 rv
+| bsem_ref : forall vm m e vm' m' vm'' m'' v fid l ofs t g ct g' i',
+             bsem_expr vm m e m' vm' v ->
+             transBeePL_type t g = Res ct g' i' ->
+             (gensym ct) = ret fid ->
+             bind_variables ge vm m ({| vname := fid; vtype := t|} :: nil) (v :: nil) m' ->
+             bsem_expr vm' m' (Var {| vname := fid; vtype := t |}) m'' vm'' (Vloc l ofs) -> 
+             bsem_expr vm m (Prim Ref [:: e] t) m'' vm'' (Vloc l ofs)
+| bsem_deref : forall vm m e t m' vm' l ofs bf v,
+               bsem_expr vm m e m' vm' (Vloc l ofs) ->
+               deref_addr ge (typeof_expr e) m l ofs bf v ->
+               typeof_expr e = t ->
+               BeeTypes.type_is_volatile t = false ->
+               bsem_expr vm m (Prim Deref (e :: nil) t) m' vm' v
+| bsem_massgn : forall vm m e1 m' vm' l ofs bf e2 vm'' m'' v v' t g1 ct1 ct2 g2 i g3 i',  
+                bsem_expr vm m e1 m' vm' (Vloc l ofs) ->
+                bsem_expr vm' m' e2 vm'' m'' v ->
+                transBeePL_type (typeof_expr e1) g1 = Res ct1 g2 i ->
+                transBeePL_type (typeof_expr e2) g2 = Res ct2 g3 i' ->
+                sem_cast (transBeePL_value_cvalue v) ct2 ct1 m = Some (transBeePL_value_cvalue v') ->
+                assign_addr ge (typeof_expr e1) m l ofs bf v' m' v' -> 
+                typeof_expr e1 = t ->
+                bsem_expr vm m (Prim Massgn (e1 :: e2 :: nil) t) vm'' m'' v'
+| bsem_uop : forall vm m e v uop m' vm' v' t ct v'' g g' i,
+             bsem_expr vm m e m' vm' v ->
+             transBeePL_type (typeof_expr e) g = Res ct g' i ->
+             sem_unary_operation uop (transBeePL_value_cvalue v) ct m' = Some v' ->
+             transC_val_bplvalue v' = OK v'' ->
+             bsem_expr vm m (Prim (Uop uop) (e :: nil) t) m' vm' v''
+| bsem_bop : forall cenv vm m e1 e2 t v1 v2 bop vm' m' m'' vm'' v ct1 ct2 v' g g' i g'' i',
+             bsem_expr vm m e1 m' vm' v1 ->
+             bsem_expr vm' m' e2 m'' vm'' v2 ->
+             transBeePL_type (typeof_expr e1) g = Res ct1 g' i ->
+             transBeePL_type (typeof_expr e2) g' = Res ct2 g'' i'->
+             sem_binary_operation cenv bop (transBeePL_value_cvalue v1) ct1 
+                                           (transBeePL_value_cvalue v2) ct2 m'' = Some v ->
+             transC_val_bplvalue v = OK v' ->
+             bsem_expr vm m (Prim (Bop bop) (e1 :: e2 :: nil) t) m'' vm'' v'
+(* fix me : add semantics for run primitive *)
+| bsem_bind : forall vm m x e1 vm' m' v m'' vm'' e2 e2' m''' v' tx t,
+              bsem_expr vm m e1 m' vm' v -> 
+              subst ge vm' m' x v e2 m'' e2' ->
+              bsem_expr vm' m'' e2' m''' vm'' v' ->
+              bsem_expr vm m (Bind x tx e1 e2 t) m''' vm'' v'
+| bsem_ctrue : forall vm m e1 e2 e3 t vm' m' vb g ct1 g' i v vm'' m'', 
+               bsem_expr vm m e1 m' vm' vb -> 
+               transBeePL_type (typeof_expr e1) g = Res ct1 g' i ->
+               bool_val (transBeePL_value_cvalue vb) ct1 m' = Some true ->
+               bsem_expr vm' m' e2 m'' vm'' v ->
+               bsem_expr vm m (Cond e1 e2 e3 t) m'' vm'' v
+| bsem_cfalse : forall vm m e1 e2 e3 t vm' m' vb g ct1 g' i v vm'' m'', 
+                bsem_expr vm m e1 m' vm' vb -> 
+                transBeePL_type (typeof_expr e1) g = Res ct1 g' i ->
+                bool_val (transBeePL_value_cvalue vb) ct1 m' = Some false ->
+                bsem_expr vm' m' e3 m'' vm'' v ->
+                bsem_expr vm m (Cond e1 e2 e3 t) m'' vm'' v
+| bsem_ut : forall vm m, 
+            bsem_expr vm m (Unit (Ptype Tunit)) m vm Vunit
+| bsem_adr : forall vm m l ofs,
+              bsem_expr vm m (Addr l ofs) m vm (Vloc l.(lname) ofs)
+| bsem_eapp : forall vm m es vm' m' m'' vs ef g cef g' i' vres bv ts ty t,
+              bsem_exprs vm m es m' vm' vs ->
+              befuntion_to_cefunction ef g = Res cef g' i' ->
+              external_call cef ge (transBeePL_values_cvalues vs) m' t vres m'' ->
+              transC_val_bplvalue vres = OK bv ->
+              bsem_expr vm m (BeePL.Eapp ef ts es ty) m'' vm' bv
+(* fix me : add semantics for hexpr *)
+with bsem_exprs : vmap -> Memory.mem -> list BeePL.expr -> Memory.mem -> vmap -> list value -> Prop :=
+| bsem_nil : forall vm m,
+             bsem_exprs vm m nil m vm nil
+| bsem_cons : forall vm m m' m'' v vs e es vm' vm'',
+              bsem_expr vm m e m' vm' v ->
+              bsem_exprs vm' m' es m'' vm'' vs ->
+              bsem_exprs vm m (e :: es) m'' vm'' (v :: vs). 
+
+End Big_Step_Semantics.
+
+Definition is_value (e : BeePL.expr) : bool :=
+match e with 
+| Val _ _ => true 
+| _ => false
+end.
+
+(** An expr is safe if it cannot get stuck by doing any transition - 
+    Either it reaches a value or it takes step **)
+Definition safe_expr (bge : genv) (e : BeePL.expr) : Prop :=
+forall v vm m vm' m', bsem_expr bge vm m e vm' m' v.
